Var bindings, query output etc
Signed-off-by: Anand Krishnamoorthi <anakrish@microsoft.com>

Rego.Interpreter.fst
@@ -14,9 +14,25 @@ let make_new () = {
    loop_exprs = [];
 }
 
-let rec eval_expr (e:expr) (i:intr)  : Tot (value*intr) 
-//(decreases expr)
+let lookup_loop_var (i:intr) (e:expr) =
+    List.Tot.find (fun (k,_) -> k = e) i.loop_exprs
+
+let rec lookup_var_in_scopes (scopes:list scope) (name:string) =
+    match scopes with
+    | hd::tl ->
+      (match List.Tot.find (fun (n,_) -> n = name) hd with
+      | Some (_, v) -> v
+      | None -> lookup_var_in_scopes tl name)
+    | _ -> Undefined
+
+let lookup_local_var (i:intr) (name:string) =
+    lookup_var_in_scopes i.scopes name
+
+let rec eval_expr (e:expr) (i:intr)  : Tot (value*intr)
 =
+  match lookup_loop_var i e with
+  | Some((_, v)) -> (v, i)
+  | None ->
   match e with
   | Var v -> lookup_var v i
   | Value v -> (v, i)
@@ -26,59 +42,58 @@ let rec eval_expr (e:expr) (i:intr)  : Tot (value*intr)
   | Ast.ArrayCompr query -> eval_query_stmts query.stmts (Value.Array []) i
   | Ast.SetCompr query -> eval_query_stmts query.stmts (Value.Set []) i
   | Ast.ObjectCompr query -> eval_query_stmts query.stmts (Value.Object []) i
+  | Ast.RefDot (refr, field) -> eval_ref_dot refr (field, i)
+  | Ast.RefBrack (refr, index) -> eval_ref_brack (refr, index) i
+  | Ast.AssignExpr (op, lhs, rhs) -> eval_assign_expr (op, lhs, rhs) i
   | _ -> (Undefined, i)
 
+
 and eval_array_elems (elems:list expr) (values:list value) (i:intr)  : Tot (value*intr)
-(decreases elems)
 =
   match elems with
   | [] -> (Value.Array (List.Tot.rev values), i)
-  | hd::tl -> 
+  | hd::tl ->
     match eval_expr hd i with
     | (Undefined, i') -> (Undefined, i')
     | (v, i') -> eval_array_elems tl (v::values) i'
 
 and eval_set_elems (elems:list expr) (values:list value) (i:intr)  : Tot (value*intr)
-(decreases elems)
 =
   match elems with
   | [] -> (List.Tot.fold_left Value.insert_into_set (Value.Set []) values, i)
-  | hd::tl -> 
+  | hd::tl ->
     match eval_expr hd i with
     | (Undefined, i') -> (Undefined, i')
     | (v, i') -> eval_set_elems tl (v::values) i'
 
 and eval_fields (fields:list (expr*expr)) (obj:value) (i:intr)  : Tot (value*intr)
-(decreases fields)
 =
   match fields with
   | [] -> (obj, i)
-  | (key_expr,value_expr)::tl -> 
+  | (key_expr,value_expr)::tl ->
     match eval_expr key_expr i with
     | (Undefined, i') -> (Undefined, i')
-    | (kv, i') -> 
+    | (kv, i') ->
       match eval_expr value_expr i' with
       | (Undefined, i'') -> (Undefined, i'')
       | (vv, i'') -> eval_fields tl (insert_into_object obj kv vv) i''
-  
-and lookup_var (ident:string) (i:intr)  : Tot (value*intr) 
-(decreases ident) 
-=
-  (Undefined, i)
 
-and eval_query_stmts (stmts:list literalStmt) (out:value) (i:intr) : Tot (value*intr) 
-(decreases stmts)
+and lookup_var (ident:string) (i:intr)  : Tot (value*intr)
+=
+  (lookup_local_var i ident, i)
+
+and eval_query_stmts (stmts:list literalStmt) (out:value) (i:intr) : Tot (value*intr)
 =
   match stmts with
   | hd::[] ->
     (match hd.literal with
-    | ArrayComprOutput e -> 
+    | ArrayComprOutput e ->
       let (v, i') = eval_expr e i in
       (insert_into_array out v, i')
-    | SetComprOutput e -> 
+    | SetComprOutput e ->
       let (v, i') = eval_expr e i in
       (insert_into_set out v, i')
-    | ObjectComprOutput (ke, ve) -> 
+    | ObjectComprOutput (ke, ve) ->
       let (kv, i') = eval_expr ke i in
       let (vv, i'') = eval_expr ve i' in
       (insert_into_object out kv vv, i')
@@ -87,9 +102,46 @@ and eval_query_stmts (stmts:list literalStmt) (out:value) (i:intr) : Tot (value*
     let (v, i') = match hd.literal with
     | Expr e -> eval_expr e i
     | _ -> (Undefined, i)
-    in eval_query_stmts tl out i' 
+    in eval_query_stmts tl out i'
   | [] -> (Undefined, i)
- 
+
+(* todo chaining *)
+and eval_ref_dot (refr:expr) pr  : Tot (value*intr)
+=
+    let (field, i) = pr in
+    let (v, i') = eval_expr refr i in
+    (lookup_path v (Value.String field::[]), i')
+
+(* todo chaining *)
+and eval_ref_brack (pr:expr*expr) (i:intr)  : Tot (value*intr)
+=
+    let (refr, index) = pr in
+    let (v, i') = eval_expr refr i in
+    let (idx, i'') = eval_expr index i' in
+    (lookup_path v (idx::[]), i'')
+
+(* todo...actual implementation is quite complex *)
+and eval_assign_expr (t: (assignOp*expr*expr)) (i:intr) : Tot (value*intr)
+=
+  let (_, lhs, rhs) = t in
+  match lhs with
+  | Var name ->
+    (
+      let (rv, i') = eval_expr rhs i in
+      match rv with
+      | Undefined -> (Undefined, i')
+      | _ -> (* todo check existing binding *)
+        match i'.scopes with
+        | hd::tl -> (Bool true, {i' with scopes = ((name, rv)::hd)::tl})
+        | _ -> (Undefined, i')
+    )
+  | _ -> (Undefined, i)
+
+
+
 let eval (i:intr) (e:Ast.expr) : (value*intr) =
   eval_expr e i
 
+let eval_user_query (i:intr) (q:Ast.query) : (value*intr) =
+  let i' = { i with scopes = []::i.scopes } in
+  eval_query_stmts q.stmts (Value.Array []) i'
